



# Equations

## Expanding Brackets

1  $3(a - 6) = 8$

2  $8(a - 2) = 20$

3  $5(a + 7) = 45$

4  $9(a - 1) = 18$

5  $6(2a + 3) = 30a$

6  $7(a - 3) = 2(a + 7)$

7  $6(b + 2) = 4(b + 5)$

8  $5(2b - 3) = 7(b + 3)$

9  $3(a + 6) = a + 22$

10  $7m - 4 = 3(m + 4)$

11  $4(5 - b) = b$

12  $6(n + 2) = 4n + 15$

13  $2(3a - 7) + 4 = 3(a + 2) + 2$

14  $5a - (1 - 2a) = 5 - 3(1 + a)$

15  $4(b - 1) - 3(b - 2) = 4 - 5b$

## Answers

1  $a = 6\frac{2}{3}$

2  $a = 4\frac{1}{2}$

3  $a = 2$

4  $a = 3$

5  $a = 1$

6  $a = 7$

7  $b = 4$

8  $b = 12$

9  $a = 2$

10  $m = 4$

11  $b = 4$

12  $n = 15$

13  $a = 6$

14  $a = \frac{3}{10}$

15  $b = \frac{1}{3}$

